zoo_saturn/spmc_queue: Specify.

theories/zoo_saturn/spmc_queue.v
@@ -1,5 +1,11 @@
 From zoo Require Import
   prelude.
+From zoo.language Require Import
+  notations.
+From zoo.diaframe Require Import
+  diaframe.
+From zoo_std Require Import
+  option.
 From zoo_saturn Require Export
   base
   spmc_queue__code.
@@ -7,6 +13,114 @@ From zoo_saturn Require Import
   spmc_queue__types.
 From zoo Require Import
   options.
+
+Implicit Types v t : val.
+
+Class SpmcQueueG Σ `{zoo_G : !ZooG Σ} := {
+}.
+
+Definition spmc_queue_Σ := #[
+].
+#[global] Instance subG_spmc_queue_Σ Σ `{zoo_G : !ZooG Σ} :
+  subG spmc_queue_Σ Σ →
+  SpmcQueueG Σ.
+Proof.
+  (* solve_inG. *)
+Qed.
+
+Section spmc_queue_G.
+  Context `{spmc_queue_G : SpmcQueueG Σ}.
+
+  Parameter spmc_queue_inv : val → namespace → iProp Σ.
+
+  Parameter spmc_queue_model : val → list val → iProp Σ.
+
+  Parameter spmc_queue_producer : val → list val → iProp Σ.
+
+  #[global] Instance spmc_queue_model_timeless t vs :
+    Timeless (spmc_queue_model t vs).
+  Proof.
+  Admitted.
+  #[global] Instance spmc_queue_producer_timeless t ws :
+    Timeless (spmc_queue_producer t ws).
+  Proof.
+  Admitted.
+  #[global] Instance spmc_queue_inv_persistent t ι :
+    Persistent (spmc_queue_inv t ι).
+  Proof.
+  Admitted.
+
+  Lemma spmc_queue_producer_valid t vs ws :
+    spmc_queue_model t vs -∗
+    spmc_queue_producer t ws -∗
+    ⌜vs `suffix_of` ws⌝.
+  Proof.
+  Admitted.
+
+  Lemma spmc_queue_create_spec ι :
+    {{{
+      True
+    }}}
+      spmc_queue_create ()
+    {{{ t,
+      RET t;
+      spmc_queue_inv t ι ∗
+      spmc_queue_model t [] ∗
+      spmc_queue_producer t []
+    }}}.
+  Proof.
+  Admitted.
+
+  Lemma spmc_queue_is_empty_spec t ι :
+    <<<
+      spmc_queue_inv t ι
+    | ∀∀ vs,
+      spmc_queue_model t vs
+    >>>
+      spmc_queue_is_empty t @ ↑ι
+    <<<
+      spmc_queue_model t vs
+    | RET #(bool_decide (vs = []%list));
+      True
+    >>>.
+  Proof.
+  Admitted.
+
+  Lemma spmc_queue_push_spec t ι ws v :
+    <<<
+      spmc_queue_inv t ι ∗
+      spmc_queue_producer t ws
+    | ∀∀ vs,
+      spmc_queue_model t vs
+    >>>
+      spmc_queue_push t v @ ↑ι
+    <<<
+      spmc_queue_model t (vs ++ [v])
+    | RET ();
+      spmc_queue_producer t (vs ++ [v])
+    >>>.
+  Proof.
+  Admitted.
+
+  Lemma spmc_queue_pop_spec t ι :
+    <<<
+      spmc_queue_inv t ι
+    | ∀∀ vs,
+      spmc_queue_model t vs
+    >>>
+      spmc_queue_pop t @ ↑ι
+    <<<
+      spmc_queue_model t (tail vs)
+    | RET head vs;
+      True
+    >>>.
+  Proof.
+  Admitted.
+End spmc_queue_G.
+
+#[global] Opaque spmc_queue_inv.
+#[global] Opaque spmc_queue_model.
+#[global] Opaque spmc_queue_producer.
 
 #[global] Opaque spmc_queue_create.
 #[global] Opaque spmc_queue_is_empty.
